sep tactic

SL/Assertions.thy
@@ -1,5 +1,5 @@
 theory Assertions
-  imports "../Algebra/BBI" Heap
+  imports "../Algebra/BBI" Heap "$ISABELLE_HOME/src/HOL/Eisbach/Eisbach"
 begin
 
 no_notation 
@@ -8,23 +8,29 @@ no_notation
 
 type_synonym 'a pred = "('a \<times> heap) set"
 
+(*****************************************************************************************)
+section {* Separation Conjunction *}
+(*****************************************************************************************)
+
 definition emp :: "'a pred" where
   "emp \<equiv> {(s, h). h = Map.empty}"
 
 definition sep :: "'a pred \<Rightarrow> 'a pred \<Rightarrow> 'a pred" (infixl "*" 80) where
   "p * q \<equiv> {(s, h1 ++ h2) | s h1 h2. h1 \<bottom> h2 \<and> (s, h1) \<in> p \<and> (s, h2) \<in> q}" 
 
-lemma sep_assoc: "p * (q * r) = (p * q) * r"
+lemma sep_assoc: "(p * q) * r = p * (q * r)"
   apply (auto simp: sep_def)
-  using Heap.pmult_def_eq apply blast
-  using Heap.pmult_ab1 Heap.pmult_ab2 Heap.pmult_ab_assoc by blast
+  using Heap.pmult_ab1 Heap.pmult_ab2 Heap.pmult_ab_assoc apply blast
+  using Heap.pmult_def_eq by blast
 
 lemma sep_comm: "p * q = q * p"
   apply (auto simp: sep_def)
   using Heap.pmult_comm Heap.pmult_comm_def apply blast
   using Heap.pmult_comm Heap.pmult_comm_def by blast
 
+(*****************************************************************************************)
 section {* Algebraic structure *}
+(*****************************************************************************************)
 
 interpretation bbi!: bbi Inf Sup inf less_eq less sup bot top minus uminus sep emp
   apply default
@@ -40,7 +46,7 @@ abbreviation (input)
   constants :: "'b \<Rightarrow> ('a \<Rightarrow> 'b)" ("#_") where
   "#x \<equiv> \<lambda>_. x"
 
-abbreviation (input) 
+abbreviation 
   pred_ex :: "('b \<Rightarrow> 'a set) \<Rightarrow> 'a set" (binder "EXS " 10) where
   "EXS x. P x \<equiv> {s. \<exists>x. s \<in> P x}"
 
@@ -52,15 +58,18 @@ abbreviation (input)
   pred_eq :: "('a \<Rightarrow> 'b) \<Rightarrow> ('a \<Rightarrow> 'b) \<Rightarrow> 'a pred" (infix "\<Midarrow>" 50) where
   "e \<Midarrow> e' \<equiv> {(s, h). e s = e' s}"
 
-no_notation residual_r (infixr "\<rightarrow>" 60)
-abbreviation (input) 
-  pred_impl :: "'a pred \<Rightarrow> 'a pred \<Rightarrow> 'a pred" (infix "\<rightarrow>" 60) where
-  "p \<rightarrow> q \<equiv> (-p) \<squnion> q"
+abbreviation true :: "'a pred" where
+  "true \<equiv> \<top>"
 
-lemma sexI: "P x \<le> (EXS x. P x)"
-  by auto
+abbreviation false :: "'a pred" where
+  "false \<equiv> {}"
 
+definition pure_pred :: "'a set \<Rightarrow> 'a pred" ("<_>") where
+  "<P> \<equiv> {(s, h). s \<in> P} \<sqinter> emp"
+
+(*****************************************************************************************)
 section {* Variables and Expressions *}
+(*****************************************************************************************)
 
 type_synonym ('v, 's) exp = "'s \<Rightarrow> 'v"
 type_synonym 'a nat_exp = "'a \<Rightarrow> nat"
@@ -89,19 +98,42 @@ abbreviation vars2 :: "('v, 's) lval \<Rightarrow> ('v, 's) rval \<Rightarrow> (
 abbreviation vars3 :: "('v, 's) lval \<Rightarrow> ('v, 's) rval \<Rightarrow> bool" where
   "vars3 u_upd v \<equiv> \<forall>s t. v (u_upd (\<lambda>_. t s) s) = v s"
 
-abbreviation subst_pred :: "('s \<times> 'h) set \<Rightarrow> ('v, 's) lval \<Rightarrow> ('v, 's) rval \<Rightarrow> ('s \<times> 'h) set" where
+definition subst_pred :: "('s \<times> 'h) set \<Rightarrow> ('v, 's) lval \<Rightarrow> ('v, 's) rval \<Rightarrow> ('s \<times> 'h) set" where
   "subst_pred P u t \<equiv> Collect (\<lambda>(s, h). (u (\<lambda>_. t s) s, h) \<in> P)"
 
-abbreviation free_pred :: "('v, 's) lval \<Rightarrow> 's pred \<Rightarrow> bool" where
+abbreviation subst_pred_s :: "'s set \<Rightarrow> ('v, 's) lval \<Rightarrow> ('v, 's) rval \<Rightarrow> 's set" where
+  "subst_pred_s P u t \<equiv> Collect (\<lambda>s. (u (\<lambda>_. t s) s) \<in> P)"
+
+abbreviation (input) free_pred :: "('v, 's) lval \<Rightarrow> 's pred \<Rightarrow> bool" where
   "free_pred v R \<equiv> \<forall>t. R = subst_pred R v t"
 
+(*****************************************************************************************)
+section {* Substitution Lemmas *}
+(*****************************************************************************************)
+
+named_theorems spred
+
+lemma subst_inf [spred]: "subst_pred (P \<sqinter> Q) i_update j = (subst_pred P i_update j) \<sqinter> (subst_pred Q i_update j)"
+  by (auto simp: subst_pred_def)
+
+lemma subst_sep [spred]: "subst_pred (P * Q) i_update j = (subst_pred P i_update j) * (subst_pred Q i_update j)"
+  by (auto simp: subst_pred_def sep_def)
+
+lemma subst_wand [spred]: "subst_pred (P -* Q) i_update j = (subst_pred P i_update j) -* (subst_pred Q i_update j)"
+  oops
+
+lemma subst_exs [spred]: "subst_pred (EXS k. (P k)) i_update j = (EXS k. (subst_pred (P k) i_update j))"
+  by (auto simp: subst_pred_def)
+
+(*****************************************************************************************)
 section {* Predicates over the Heaplet Model*}
+(*****************************************************************************************)
 
 definition singleton :: "'a nat_exp \<Rightarrow> 'a nat_exp \<Rightarrow> 'a pred" ("_ \<mapsto> _" [50, 50] 60) where
   "e \<mapsto> e' \<equiv> {(s, h). h = [e s \<mapsto> e' s]}"
 
 definition any_singleton :: "'a nat_exp \<Rightarrow> 'a pred" ("_ \<mapsto> -" [50] 60) where
-  "e \<mapsto> - \<equiv> EXS e'. e \<mapsto> e'"
+  "e \<mapsto> - \<equiv> EXS e'. e \<mapsto> #e'"
 
 definition points_to :: "'a nat_exp \<Rightarrow> 'a nat_exp \<Rightarrow> 'a pred" ("_ \<hookrightarrow> _" [50, 50] 60) where
   "e \<hookrightarrow> e' \<equiv> (e \<mapsto> e') * \<top>"
@@ -111,6 +143,22 @@ definition any_points_to :: "'a nat_exp \<Rightarrow> 'a pred" ("_ \<hookrightar
 
 definition doublet :: "'a nat_exp \<Rightarrow> 'a nat_exp \<Rightarrow> 'a nat_exp \<Rightarrow> 'a pred" ("_ \<mapsto> _, _" [50, 50, 50] 60) where
   "e \<mapsto> e1, e2 \<equiv> (e \<mapsto> e1) * ((\<lambda>s. plus (e s) 1) \<mapsto> e2)"
+
+lemma subst_singleton [spred]: "subst_pred (x \<mapsto> y) i_update j = (subst x i_update j \<mapsto> subst y i_update j)"
+  by (auto simp: subst_pred_def singleton_def)
+
+lemma subst_any_singleton [spred]: "subst_pred (x \<mapsto> -) i_update j = (subst x i_update j \<mapsto> -)"
+  by (auto simp: subst_pred_def any_singleton_def singleton_def)
+
+lemma subst_doublet [spred]: "subst_pred (x \<mapsto> y, z) i_update j = (subst x i_update j \<mapsto> subst y i_update j, subst z i_update j)"
+  by (simp add: doublet_def spred)
+
+lemma subst_no_state [spred]: "subst_pred {(s, h). P} i_update j = {(s, h). P}"
+  by (simp add: subst_pred_def)
+
+(*****************************************************************************************)
+section {* Arbitrary Lemmas *}
+(*****************************************************************************************)
 
 lemma wand_eq: "{(s, h). \<forall>h'. h \<bottom> h' \<and> (s, h') \<in> P \<longrightarrow> (s, h ++ h') \<in> Q} \<le> P -* Q"
   apply (rule bbi.sep_implI1)
@@ -166,5 +214,398 @@ lemma reynolds5: "(e \<hookrightarrow> e') \<sqinter> p \<le> (e \<mapsto> e') *
   apply (erule_tac x=h2 in allE)
   apply auto
   by (simp add: domIff map_add_upd_left)
+
+lemma reynolds5': "P \<le> (e \<mapsto> e') * true \<Longrightarrow> P \<le> Q \<Longrightarrow> P \<le> (e \<mapsto> e') * ((e \<mapsto> e') -* Q)"
+  apply (rule order_trans[rotated])
+  apply (rule reynolds5)
+  apply (auto simp: points_to_def)
+done
+  
+
+
+(*****************************************************************************************)
+section {* Lists *}
+(*****************************************************************************************)
+
+abbreviation (input) is_nil :: "'a nat_exp \<Rightarrow> 'a pred" ("_ \<Midarrow> nil") where
+  "i \<Midarrow> nil \<equiv> {(s, h). i s \<notin> dom h}"
+
+primrec list_seg :: "nat list \<Rightarrow> 'a nat_exp \<Rightarrow> 'a nat_exp \<Rightarrow> 'a pred" where
+  "list_seg [] i j = emp \<sqinter> (i \<Midarrow> j)"
+| "list_seg (x#xs) i k = (EXS j. (i \<mapsto> #x, #j) * list_seg xs #j k)"
+
+lemma list_seg_empty: "list_seg [] i j = <{s. i s = j s}>"
+  by (auto simp: pure_pred_def)
+
+lemma singleton_list [simp]: "(list_seg [x] i j) = (i \<mapsto> #x, j)"
+  by (auto simp: sep_def doublet_def singleton_def emp_def)
+
+lemma list_seg_exs: "(EXS j. (emp \<sqinter> (i \<Midarrow> j)) * list_seg ys j k) = list_seg ys i k"
+  apply (auto simp: sep_def doublet_def singleton_def emp_def)
+  apply (induct ys)
+  apply (auto simp: doublet_def singleton_def sep_def)
+done
+
+lemma list_seg_merge: "(list_seg (xs@ys) i k) = (EXS j. (list_seg xs i j) * (list_seg ys j k))"
+  apply (induct xs arbitrary: i)
+  apply (simp add: list_seg_exs)
+  apply (auto simp: sep_def doublet_def singleton_def emp_def ortho_def)
+  oops
+
+lemma list_seg_rev: "(list_seg (xs@[x]) i k) = (EXS j. (list_seg xs i j) * (j \<mapsto> #x, k))"
+  oops
+
+lemma "list_seg xs i j \<le> -(i \<Midarrow> nil) \<squnion> ((#xs \<Midarrow> #[]) \<sqinter> (i \<Midarrow> nil))"
+  apply (induct xs)
+  apply clarsimp
+  apply (auto simp: sep_def doublet_def singleton_def emp_def ortho_def)
+done
+
+lemma "list_seg xs i j \<le> (i \<Midarrow> j) \<squnion> - (#xs \<Midarrow> #[])"
+  apply (induct xs)
+  apply clarsimp
+  apply (auto simp: sep_def doublet_def singleton_def emp_def ortho_def)
+done
+
+lemma subst_list_seg [spred]: "subst_pred (list_seg xs m n) i_update j = list_seg xs (subst m i_update j) (subst n i_update j)"
+  apply (induct xs arbitrary: m n)
+  apply (force simp: subst_pred_def emp_def)
+  apply (auto simp: spred)
+done
+
+no_notation sup (infixl "+" 65)
+
+lemma exs1: "(EXS j. (i \<mapsto> a, #j) * P j) = (i \<mapsto> a) * (EXS j. ((\<lambda>s. i s + 1) \<mapsto> #j) * P j)"
+  apply (auto simp: sep_def doublet_def singleton_def emp_def ortho_def)
+  apply (erule_tac x="[Suc (i s) \<mapsto> x] ++ h2" in allE)
+  apply auto
+done
+(*
+lemma "list_seg [] i j = <{s. i s = j s}>"
+  by (auto simp: state_pred_def emp_def)
+*)
+
+definition llist :: "nat list \<Rightarrow> 'a nat_exp \<Rightarrow> 'a pred" where
+  "llist xs i \<equiv> list_seg xs i #0 \<sqinter> {(s, h). 0 \<notin> dom h}"
+
+lemma llist_empty_var: "llist [] i = (i \<Midarrow> #0) \<sqinter> emp"
+  by (auto simp add: llist_def emp_def)
+
+lemma llist_empty: "llist [] i = <{s. i s = 0}>"
+  by (auto simp add: llist_def pure_pred_def emp_def)
+
+lemma llist_empty_zero: "llist [] (\<lambda>s. 0) = emp"
+  by (auto simp add: llist_def emp_def)
+
+lemma llist_simp2: "llist (Cons x xs) i = <{s. i s \<noteq> 0}> * (EXS k. (i \<mapsto> #x, #k) * llist xs #k)"
+  apply (auto simp: llist_def sep_def doublet_def singleton_def pure_pred_def emp_def)
+  apply auto
+  using neq0_conv apply fastforce
+done
+
+lemma llist_simp3: "llist (Cons x xs) i = -(i \<Midarrow> #0) \<sqinter> (EXS k. (i \<mapsto> #x, #k) * llist xs #k)"
+  apply (auto simp: llist_def sep_def doublet_def singleton_def)
+  apply (rule_tac x=xa in exI)
+  apply auto
+done
+
+lemma subst_llist [spred]: "subst_pred (llist xs m) i_update j = llist xs (subst m i_update j)"
+  apply (simp add: llist_def spred)
+  apply (simp add: subst_pred_def)
+
+done
+
+
+(*****************************************************************************************)
+section {* Tactics *}
+(*****************************************************************************************)
+
+
+named_theorems sep_simps
+
+lemmas [sep_simps] =
+  bbi.mult_1_left
+  bbi.mult_1_right 
+  bbi.mult_1_left
+  bbi.sep_conj_top
+  list_seg_empty
+  list_seg.simps(2)
+  doublet_def
+  llist_empty_zero
+  llist_empty
+  llist_simp2
+  points_to_def
+  any_singleton_def
+  any_points_to_def
+
+lemma [sep_simps]: "true * p = p * true"
+  by (simp add: sep_comm)
+
+lemma [sep_simps]: "<p> * <q> = <p \<sqinter> q>"
+  by (auto simp: pure_pred_def emp_def sep_def)
+
+lemma [sep_simps]: "<p> * (<q> * r) = <p \<sqinter> q> * r"
+  by (auto simp: pure_pred_def emp_def sep_def)
+
+lemma [sep_simps]: "p * <q>  = <q> * p"
+  by (simp add: sep_comm)
+
+lemma [sep_simps]: "q * (<p> * r) = <p> * (q * r)"
+  by (auto simp: pure_pred_def emp_def sep_def)
+
+lemma [sep_simps]: "x * y * z = x * (y * z)"
+  by (simp add: sep_assoc)
+
+lemma [sep_simps]: "(EXS x. P x) * Q = (EXS x. P x * Q)"
+  by (auto simp: sep_def)
+
+lemma exs [sep_simps]: "P * (EXS x. Q x) = (EXS x. P * Q x)"
+  by (auto simp: sep_def)
+
+named_theorems cancel_same
+
+lemma [cancel_same]: "p \<subseteq> q \<Longrightarrow> e = e' \<Longrightarrow> (i \<mapsto> e) * p \<subseteq> (i \<mapsto> e') * q"
+  by (simp add: bbi.Sup.qisol)
+
+lemma [cancel_same]: "p \<subseteq> q \<Longrightarrow> e = e' \<Longrightarrow> p * (i \<mapsto> e) \<subseteq> q * (i \<mapsto> e')"
+  by (simp add: bbi.Sup.qisor)
+
+lemma [cancel_same]: "p \<subseteq> q \<Longrightarrow> xs = ys \<Longrightarrow> (list_seg xs i j) * p \<subseteq> list_seg ys i j * q"
+  by (simp add: bbi.Sup.qisol)
+
+lemma [cancel_same]: "p \<subseteq> q \<Longrightarrow> xs = ys \<Longrightarrow> p * (list_seg xs i j) \<subseteq> q * list_seg ys i j"
+  by (simp add: bbi.Sup.qisor)
+
+
+lemma [sep_simps, simp]: "<UNIV> = emp"
+  by (auto simp: pure_pred_def)
+
+named_theorems sep_same
+
+declare Set.UNIV_I [sep_same]
+
+lemma [sep_same]: "emp \<le> r \<Longrightarrow> p \<le> p * r"
+  apply (auto simp: sep_def emp_def)
+  apply (rule_tac x=b in exI)
+  apply (rule_tac x=Map.empty in exI)
+  apply auto
+done
+  
+lemma [sep_same]: "p \<subseteq> list_seg [] i i * p"
+  by (auto simp: sep_def emp_def)
+
+lemma [sep_same]: "p \<le> list_seg cs j k * q \<Longrightarrow> as@cs=bs \<Longrightarrow> list_seg as i j * p \<subseteq> list_seg bs i k * q"
+  oops  
+
+lemma [sep_same]: "p \<le> list_seg cs j k \<Longrightarrow> as@cs=bs \<Longrightarrow> list_seg as i j * p \<subseteq> list_seg bs i k"
+oops
+
+lemma aa: "(s, h) \<in> llist as i * p \<Longrightarrow> as@cs=bs \<Longrightarrow> ((s, h) \<in> p \<Longrightarrow> (s, h) \<in> llist cs j) \<Longrightarrow> (s, h) \<in> llist bs i"
+oops
+
+lemma split_conc: "P \<subseteq> Q \<Longrightarrow> P \<subseteq> <R> * true \<Longrightarrow> P \<subseteq> <R> * Q"
+  by (auto simp: sep_def pure_pred_def emp_def)
+
+lemma mono_exs: "(\<And>x s h. (s, h) \<in> P x \<Longrightarrow> (s, h) \<in> Q x) \<Longrightarrow> (EXS x. P x) \<subseteq> (EXS y. Q y)"
+  by auto
+
+lemma mono_exs2: "(\<And>x. P x \<subseteq> Q x) \<Longrightarrow> (EXS x. P x) \<subseteq> (EXS y. Q y)"
+  by auto
+
+lemma pred_conjI: "(s, h) \<in> P \<Longrightarrow> (s, h) \<in> Q \<Longrightarrow> (s, h) \<in> P \<sqinter> Q"
+  by auto
+
+lemma pred_conjE: "(s, h) \<in> P \<sqinter> Q \<Longrightarrow> ((s, h) \<in> P \<Longrightarrow> (s, h) \<in> Q \<Longrightarrow> R) \<Longrightarrow> R"
+  by auto
+
+schematic_lemma pred_exI: "P \<subseteq> Q ?x \<Longrightarrow> P \<subseteq> (EXS x. Q x)"
+  by auto
+
+lemma pred_exI2: "P x \<subseteq> (EXS x. P x)"
+  by auto
+
+lemma pred_exI': "(s, h) \<in> P x \<Longrightarrow> (s, h) \<in> (EXS x. P x)"
+  by auto
+
+lemma pred_exE: "(\<And>x. P x \<subseteq> Q) \<Longrightarrow> (EXS x. P x) \<subseteq> Q"
+  by auto
+
+lemma pred_exE': "(s, h) \<in> (EXS x. P x) \<Longrightarrow> (\<And>x. (s, h) \<in> P x \<Longrightarrow> Q) \<Longrightarrow> Q"
+  by auto
+
+
+lemma split_pure_sep: "(\<And>s h. s \<in> P \<Longrightarrow> (s, h) \<in> Q \<Longrightarrow> (s, h) \<in> R) \<Longrightarrow> <P> * Q \<subseteq> R"
+  by (auto simp: pure_pred_def emp_def sep_def)
+
+lemma split_pure_conj: "(\<And>s h. P s \<Longrightarrow> (s, h) \<in> Q \<Longrightarrow> (s, h) \<in> R) \<Longrightarrow> Q \<sqinter> {(s, h). P s} \<subseteq> R"
+  by (auto simp: pure_pred_def emp_def sep_def)
+
+lemma split_pure_neg: "(\<And>s h. \<not> P s \<Longrightarrow> (s, h) \<in> Q \<Longrightarrow> (s, h) \<in> R) \<Longrightarrow> Q - {(s, h). P s} \<subseteq> R"
+  by (auto simp: pure_pred_def emp_def sep_def)
+
+lemma split_pure_sepE: "(s, h) \<in> <P> * Q \<Longrightarrow> (s \<in> P \<Longrightarrow> (s, h) \<in> Q \<Longrightarrow> R) \<Longrightarrow> R"
+  by (auto simp: pure_pred_def emp_def sep_def)
+
+lemma split_pure_sep_nostateE: "(s, h) \<in> <{s. P}> * Q \<Longrightarrow> (P \<Longrightarrow> (s, h) \<in> Q \<Longrightarrow> (s, h) \<in> R) \<Longrightarrow> (s, h) \<in> R"
+  apply (auto simp: pure_pred_def emp_def sep_def)
+apply force
+done
+
+lemma zero: "(s, h) \<in> llist x i * R \<Longrightarrow> i s = 0 \<Longrightarrow> (x = [] \<Longrightarrow> (s, h) \<in> R \<Longrightarrow> Q) \<Longrightarrow> Q"
+  apply (induct x)
+  apply (simp add: llist_empty)
+  apply (erule split_pure_sepE)
+  apply simp
+  apply (simp add: llist_simp2)
+by (metis (no_types, lifting) CollectD bbi.mult_assoc less_numeral_extra(3) split_pure_sepE)
+
+lemma not_zero: "(s, h) \<in> llist x i * R \<Longrightarrow> i s \<noteq> 0 \<Longrightarrow> (x \<noteq> [] \<Longrightarrow> (s, h) \<in> llist (Cons (hd x) (tl x)) i * R \<Longrightarrow> Q) \<Longrightarrow> Q"
+  apply (induct x)
+  apply (simp add: llist_empty)
+  apply (erule split_pure_sepE)
+  apply simp
+  apply (simp add: llist_simp2)
+done
+
+lemma split_pureE: "(s, h) \<in> <Q> * P \<Longrightarrow> (s \<in> Q \<Longrightarrow> (s, h) \<in> P \<Longrightarrow> (s, h) \<in> R) \<Longrightarrow> (s, h) \<in> R"
+  by (auto simp: pure_pred_def sep_def emp_def)
+
+lemma split_pure_sep2: "(\<And>s h. s \<in> P \<Longrightarrow> (s, h) \<in> Q \<Longrightarrow> (s, h) \<in> R) \<Longrightarrow> <P> * Q \<subseteq> R"
+  by (auto simp: pure_pred_def emp_def sep_def)
+
+lemma split_pure_sep': "s \<in> P \<Longrightarrow> (s, h) \<in> Q \<Longrightarrow> (s, h) \<in> <P> * Q"
+  by (auto simp: pure_pred_def emp_def sep_def)
+
+lemma tt: "(s, h) \<in> (i \<mapsto> e) * P \<Longrightarrow> (s, h) \<in> (i \<hookrightarrow> e)"
+  by (auto simp: points_to_def sep_def)
+
+lemma "(EXS x. Q x \<sqinter> R x) \<subseteq> (EXS x. Q x) \<sqinter> (EXS x. R x)"
+apply auto
+done
+
+named_theorems sep_mono
+
+lemma trick : "mono (f :: 'a pred \<Rightarrow> 'a pred)"
+oops
+(*
+lemma tt2: "(s, h) \<in> P(i \<mapsto> x) \<Longrightarrow> mono P \<Longrightarrow> ((s, h) \<in> P(emp) \<Longrightarrow> (s, h) \<in> Q(true)) \<Longrightarrow> (s, h) \<in> Q(i \<hookrightarrow> x)"
+sorry
+
+lemma tt3: "(s, h) \<in> P(i \<mapsto> x) \<Longrightarrow> mono P \<Longrightarrow> ((s, h) \<in> P(emp) \<Longrightarrow> (s, h) \<in> Q(emp)) \<Longrightarrow> (s, h) \<in> Q(i \<mapsto> -)"
+sorry
+
+lemma tt4: "(s, h) \<in> P(i \<mapsto> x) \<Longrightarrow> mono P \<Longrightarrow> ((s, h) \<in> P(emp) \<Longrightarrow> (s, h) \<in> Q(emp)) \<Longrightarrow> (s, h) \<in> Q(i \<mapsto> -)"
+sorry
+
+lemma tt5: "mono P \<Longrightarrow> P(emp) \<subseteq> Q(emp) \<Longrightarrow> P(i \<mapsto> x) \<subseteq> Q(i \<mapsto> x)"
+sorry
+
+lemma tt5': "(s, h) \<in> P(i \<mapsto> x) \<Longrightarrow> mono P \<Longrightarrow> ((s, h) \<in> P(emp) \<Longrightarrow> (s, h) \<in> Q(emp)) \<Longrightarrow> (s, h) \<in> Q(i \<mapsto> x)"
+sorry
+
+lemma tt6[simp]: "i x = 0 \<Longrightarrow> ((x, y) \<in> P (llist xs i)) = ((x, y) \<in> P emp \<and> xs = [])"
+sorry
+
+
+lemma "Q \<longrightarrow> P \<Longrightarrow> Q \<Longrightarrow> P" 
+  apply (match premises in I: "Q \<longrightarrow> P" and I': Q \<Rightarrow> \<open>auto simp: I I'\<close>)
+done
+
+
+lemma bb: "P \<Longrightarrow> P = P' \<Longrightarrow> (P' \<Longrightarrow> Q) \<Longrightarrow> Q"
+by auto
+
+lemma "llist (xa @ xb) i = llist xa i * llist xb j"
+sorry
+
+*)
+method sep_normal =
+  (subst sep_simps | subst (asm) sep_simps | subst spred | subst (asm) spred | rule pred_exE)+
+
+method sep_same = 
+  (assumption 
+    | rule sep_same 
+(*    | rule trick *)
+    | sep_normal
+(*
+    | match conclusion in "(s, h) \<in> Q(i \<hookrightarrow> x)" for s h Q i x \<Rightarrow> \<open>erule tt2\<close>
+    | match conclusion in "(s, h) \<in> Q(i \<mapsto> -)" for s h Q i \<Rightarrow> \<open>erule tt3\<close>
+*)
+    )+
+(*
+method sep_auto = 
+  (
+    sep_normal?,             (* Normalize *)
+    (rule subrelI)?,        (* Subset relation introduction *)
+    ((erule pred_conjE)+)?,  (* Conjunction elimination *)
+    ((erule pred_exE)+)?,   (* Eliminate existentials in premises *)
+    ((rule pred_conjI)+)?;  (* Conjunction introduction *)
+    
+      (sep_same?,           (* Eliminate same expressions in both sides *)
+        (simp?, (erule conjE)+)?; (* Conjunction introduction *)
+        ((rule exI)+)?; (* Existential introduction *)
+        (simp?, (rule conjI)+)?; (* Conjunction introduction *)
+        sep_same? 
+      );
+     sep_normal?,
+     simp?
+    )
+*)
+(*
+record tt =
+  i :: nat
+  j :: nat
+  k :: nat
+
+
+lemma "<{s. i s = 0}> *  (EXS x xa. llist x i * llist xa j * <{s. rev xs = rev x @ xa}>) \<subseteq> llist (rev xs) j"
+apply sep_normal
+apply sep_auto
+apply (match premises in I: "i x = 0" and I':"((x, y) \<in> P (llist xs i))" for i x y P xs \<Rightarrow> \<open>rule bb[rotated], rule tt6[where y=y and P=P and xs=xs], rule I\<close>)
+apply sep_aut
+oops
+
+lemma "list_seg (Cons x xs) i k
+    \<subseteq> (EXS x. ((\<lambda>s. i s + 1) \<hookrightarrow> (\<lambda>_. x)) \<inter>
+               subst_pred ((i \<mapsto> -) * ((\<lambda>s. i s + 1) \<mapsto> -) * subst_pred (list_seg xs i k) i_update j) j_update (\<lambda>_. x))"
+apply sep_normal
+oops
+
+lemma "llist xs i \<subseteq> subst_pred (EXS x xa. llist x i * llist xa j \<inter> {(s, h). rev xs = rev x @ xa}) j_update (\<lambda>_. 0)"
+apply sep_auto
+done
+
+lemma "{(s, h). i s \<noteq> 0} \<inter> (EXS x xa. llist x i * llist xa j \<inter> {(s, h). rev xs = rev x @ xa})
+    \<subseteq> (EXS x. ((\<lambda>s. i s + 1) \<hookrightarrow> (\<lambda>_. x)) \<inter>
+               subst_pred
+                (((\<lambda>s. i s + 1) \<mapsto> -) *
+                 (((\<lambda>s. i s + 1) \<mapsto> j) -*
+                  subst_pred (subst_pred (EXS x xa. llist x i * llist xa j \<inter> {(s, h). rev xs = rev x @ xa}) i_update k) j_update i))
+                k_update (\<lambda>_. x))"
+apply sep_auto
+apply (rule subrelI)
+apply (erule pred_conjE)
+apply (erule pred_exE)+
+apply (erule pred_conjE)
+apply simp
+apply (erule conjE)
+oops
+
+hide_const i j k
+
+(* Examples *)
+lemma "list_seg xs i j * list_seg ys j k \<subseteq> list_seg (xs@ys) i k"
+
+oops
+(*
+  ((subst sep_normal)+ |
+  (rule order_trans[rotated], rule l1, rule allI, rule order_refl) | subst sep_simps )
+*)
+*)
+lemma "(EXS x. (x \<mapsto> i) * true * <{s. x s = j s}>) * (EXS x. (x \<hookrightarrow> j) * true) * emp * (k \<mapsto> i, j) * <{s. i s = j s}> \<subseteq> (EXS y :: 'a. F y) "
+
+apply sep_normal
+oops
+
 
 end
