SL/LinkedList2.thy
@@ -1,0 +1,196 @@
+theory LinkedList2
+  imports StoreHeapModel
+begin
+
+(*
+lemma tt1: "subst_pred (P * Q) i_update j = (subst_pred P i_update j) * (subst_pred Q i_update j)"
+  by (auto simp: subst_pred_def sep_def)
+
+lemma tt0: "subst_pred (P \<inter> Q) i_update j = (subst_pred P i_update j) \<inter> (subst_pred Q i_update j)"
+  by (auto simp: subst_pred_def sep_def)
+
+lemma tt2: "subst_pred (EXS k. (P k)) i_update j = (EXS k. (subst_pred (P k) i_update j))"
+  by (auto simp: subst_pred_def sep_def)
+
+lemma tt3: "subst_pred (EXS k. (P k) * (Q k)) i_update j = (EXS k. (subst_pred (P k) i_update j) * (subst_pred (Q k) i_update j))"
+  by (auto simp: subst_pred_def sep_def)
+
+lemma subst_singleton: "subst_pred (x \<mapsto> y) i_update j = (subst x i_update j \<mapsto> subst y i_update j)"
+  by (auto simp: subst_pred_def singleton_def)
+
+lemma subst_any_singleton: "subst_pred (x \<mapsto> -) i_update j = (subst x i_update j \<mapsto> -)"
+  by (auto simp: subst_pred_def any_singleton_def singleton_def)
+
+lemma subst_doublet: "subst_pred (x \<mapsto> y, z) i_update j = (subst x i_update j \<mapsto> subst y i_update j, subst z i_update j)"
+  apply (subst doublet_def)+
+  apply (subst tt1)+
+  apply (subst subst_singleton)+
+  apply (simp add:)
+done
+
+*)
+
+
+lemma [simp]: "i a = 0 \<Longrightarrow> (a, b) \<in> llist x i \<Longrightarrow> x = []"
+  apply (induct x)
+  apply simp
+  apply (simp add: llist_simp2)
+done
+
+lemma subst_llist [spred]: "subst_pred (llist xs m) i_update j = llist xs (subst m i_update j)"
+  apply (simp add: llist_def spred)
+  apply (simp add: subst_pred_def)
+done
+
+
+lemma [simp]: "{(s, h). True} = \<top>"
+  by auto
+
+lemma [spred]: "subst_pred UNIV i_update j = UNIV"
+  by (auto simp: subst_pred_def)
+
+lemma "i a = 0  \<Longrightarrow> (a, b) \<in> list_seg x i (\<lambda>_. 0) \<Longrightarrow> x = []"
+  apply (induct x arbitrary: a b)
+  apply simp+
+  apply (auto simp: sep_def doublet_def singleton_def ortho_def)
+oops
+
+record test =
+  i :: nat
+  j :: nat
+  k :: nat
+
+lemma "ht (list_seg (Cons x xs) i k)
+    (
+      lookup j_update (\<lambda>s. (i s) + 1);
+      dispose i;
+      dispose (\<lambda>s. i s + 1);
+      assign i_update j
+    )
+    (list_seg xs i k)"
+apply hoare 
+
+apply (rule hl_classic[rotated 3])
+apply (rule sl_lookup_global[where v=j])
+prefer 6
+apply sep_normal
+apply (rule subrelI)
+apply(erule tt5')
+defer
+apply clarsimp
+apply assumption
+prefer 4
+apply sep_normal
+apply (rule split_pure)
+apply (rule pred_exI')+
+apply sep_auto
+apply (erule tt5')
+defer
+apply (erule tt5')
+defer
+apply sep_normal
+
+apply 
+apply simp
+apply sep_normal
+apply sep_aut
+
+    
+
+
+
+lemma "ht (llist xs i)(
+      assign j_update #0;
+      awhile (EXS as bs. (llist as i * llist bs j) * (#(rev xs) \<Midarrow> #((rev as) @ bs)))
+        ({(s, h). i s \<noteq> 0}) 
+        (
+          lookup k_update (\<lambda>s. i s + 1);
+          mutation (\<lambda>s. i s + 1) j;
+          assign j_update i;
+          assign i_update k
+        )
+      )(llist (rev xs) j)"
+apply hoar
+apply sep_auto
+apply sep_auto
+prefer 3
+
+
+
+apply (rule hl_post[where Q' = "EXS x as bs. ((i \<mapsto> #x, j) * llist as k * llist bs j) \<sqinter> (#(rev xs) \<Midarrow> #((rev (x#as)) @ bs))"])
+apply (rule mptran)+
+apply sep_auto
+defer
+
+  apply (rule hl_seq)
+  apply (rule mptran)+
+defer
+  apply (rule hl_awhile)
+  apply (rule mptran)+
+  apply (rule order_refl)
+
+prefer 3
+
+  apply (rule hl_pre)
+  defer
+  apply (rule hl_assign)
+  apply (rule order_refl)
+
+prefer 3
+  apply (subst spred)+
+  apply (rule order_trans)
+prefer 2
+  apply (rule pred_exI[where x=xs])
+  apply (rule order_trans)
+prefer 2
+  apply (rule pred_exI[where x="[]"])
+  apply (simp add: spred subst_pred_def )
+
+  apply (subst Collect_neg_eq[symmetric])
+  apply (subst Collect_conj_eq[symmetric])
+  apply clarsimp
+  apply (subgoal_tac "x=[]")
+  apply (clarsimp simp: emp_def sep_def llist_def)
+  apply (clarsimp simp: emp_def sep_def ortho_def)
+  
+
+  apply (rule hl_seq)
+  apply (rule mptran)+
+  apply (rule hl_seq)
+  apply (rule mptran)+
+  apply (rule hl_seq)
+  apply (rule mptran)+
+
+prefer 4
+  apply (rule hl_assign)
+  apply (subst spred)+
+  apply (rule order_refl)
+prefer 3
+  apply (rule hl_assign)
+  apply (subst spred)+
+  apply (rule order_refl)
+
+prefer 2
+  apply (rule hl_post[where Q' = "EXS x as bs. ((i \<mapsto> #x, j) * llist as k * llist bs j) \<sqinter> (#(rev xs) \<Midarrow> #((rev (x#as)) @ bs))"])
+  apply (rule mptran)+
+
+  apply (simp add: subst_pred_def)
+  apply clarsimp
+  apply (rule_tac x=xa in exI)
+  apply (rule_tac x="x#xb" in exI)
+  defer
+
+  apply (rule sl_mut)
+
+apply (rule hl_pre)
+defer
+apply (rule sl_lookup)
+defer
+apply (subst spred)+
+apply (simp add: subst_pred_def)
+apply clarsimp
+
+
+  
+
+end
