SL/Refinement.thy
@@ -1,0 +1,230 @@
+theory Refinement
+  imports StoreHeapModel
+begin
+
+text {* Morgan Refinement Laws *}
+
+named_theorems ref_simps
+
+definition spec :: "'a pred \<Rightarrow> 'a pred \<Rightarrow> 'a ptran"  where
+  "spec p q \<equiv> Inf {F. p \<le> F q \<and> mono F}"
+
+lemma spec_ht [ref_simps]: "ht p (spec p q) q"
+  by (auto simp: ht_def spec_def)
+
+lemma spec_char [ref_simps]: "p \<le> (spec p q) q"
+  by (auto simp: ht_def spec_def)
+
+lemma specI: "mono F \<Longrightarrow> ht p F q \<Longrightarrow> spec p q \<le> F"
+  by (auto simp: ht_def spec_def intro: Inf_lower)
+
+lemma ht_spec_eq: "mono F \<Longrightarrow> ht p F q \<longleftrightarrow> spec p q \<le> F"
+proof (auto intro: specI, simp add: ht_def)
+  assume assm: "spec p q \<le> F"
+  have "p \<le> (spec p q) q"
+    by (rule spec_char)
+  also have "... \<le> F q" using assm
+    by (auto simp: le_fun_def)
+  finally show "p \<le> F q"
+    by simp
+qed 
+
+lemma spec_mono [mptran]: "mono (spec p q)"
+  by (auto simp: spec_def intro: mptran)
+
+(***********************************************************************************************)
+
+text {* Remaining Refinement Laws for Separation Logic *}
+
+named_theorems rlaw
+
+lemma strengthen_post [rlaw]: "q' \<le> q \<Longrightarrow> spec p q \<le> spec p q'"
+  by (meson hl_post ht_def specI spec_char spec_mono)
+
+lemma weaken_pre [rlaw]: "p \<le> p' \<Longrightarrow> spec p q \<le> spec p' q"
+  by (meson dual_order.trans ht_def specI spec_char spec_mono)
+
+lemma weaken_and_strengthen [rlaw]: "p \<le> p' \<Longrightarrow> q' \<le> q \<Longrightarrow> spec p q \<le> spec p' q'"
+  by (meson dual_order.trans strengthen_post weaken_pre)
+
+lemma skip_ref: "spec true true \<le> skip"
+  by (auto simp: skip_def spec_def mono_def intro!: Inf_lower)
+
+lemma abort_ref [rlaw]: "spec false true \<le> F"
+  by (metis (no_types, hide_lams) bot.extremum bot_apply dual_order.trans ht_def ht_spec_eq mono_def)
+
+lemma magic_ref [rlaw]: "F \<le> spec true false"
+  by (metis (no_types, hide_lams) antisym_conv bot.extremum ht_def ht_spec_eq le_fun_def spec_mono strengthen_post top_greatest)
+
+lemma skip_ref_var1: "spec p true \<le> skip"
+  by (simp add: hl_skip mono_skip specI)
+
+lemma skip_ref_var2 [rlaw]: "p \<le> q \<Longrightarrow> spec p q \<le> skip"
+  using hl_skip ht_spec_eq mono_skip by blast
+
+lemma sequence_ref [rlaw]: "spec p q \<le> (spec p r); (spec r q)"
+  using hl_seq mono_seq specI spec_ht spec_mono by blast
+
+lemma choice_ref [rlaw]: "spec p q \<le> x \<Longrightarrow> spec p q \<le> y \<Longrightarrow> spec p q \<le> x \<sqinter> y"
+  by simp
+
+lemma test_expl_ref [rlaw]: "spec p q \<le>  \<lfloor>b\<rfloor>; (spec (p \<sqinter> b) q)"
+  by (metis hl_asumption ht_def inf_commute mono_assumption mono_seq seq_def specI spec_char spec_mono)
+
+lemma test_expr_ref [rlaw]: "spec p (q \<sqinter> b) \<le> (spec p q); \<lfloor>b\<rfloor>"
+  by (metis Assertions.bbi.join_meet_galois Sup.order_refl assumption_def hl_seq ht_def inf_commute mono_assumption mono_seq specI spec_char spec_mono)
+
+lemma conditional_ref [rlaw]: "spec p q \<le> cond b (spec (p \<sqinter> b) q) (spec (p \<sqinter> -b) q)"
+  by (metis hl_cond ht_def inf_commute mono_cond specI spec_char spec_mono)
+
+lemma while_ref [rlaw]: "spec p (p \<sqinter> -b) \<le> while b (spec (p \<sqinter> b) p)"
+  by (metis hl_while ht_def inf_commute mono_while specI spec_char spec_mono)
+
+lemma assignment_ref [rlaw]: "p \<subseteq> subst_pred q v m \<Longrightarrow> spec p q \<le> assign v m"
+  by (auto simp: subst_pred_def assign_def spec_def basic_def valid_mem_def intro!: Inf_lower mptran)
+
+lemma following_ref: "mono y \<Longrightarrow> x \<le> y ; z \<Longrightarrow> z \<le> w \<Longrightarrow> x \<le> y ; w"
+proof -
+  assume m: "mono y" and zw: "z \<le> w" and "x \<le> y ; z"
+  hence "x \<le> y ; z"
+    by simp
+  also have "... \<le> y ; w"
+    apply (simp add: seq_def)
+    apply (rule le_funI)
+    apply simp
+    apply (rule monoD, rule m)
+    using zw by (auto simp: le_fun_def)
+  finally show ?thesis
+    by simp
+qed
+
+lemma leading_ref: "x \<le> y ; w \<Longrightarrow> y \<le> z \<Longrightarrow> x \<le> z ; w"
+proof -
+  assume zw: "y \<le> z" and "x \<le> y ; w"
+  hence "x \<le> y ; w"
+    by simp
+  also have "... \<le> z ; w"
+    using zw by (auto simp: seq_def le_fun_def)
+  finally show ?thesis
+    by simp
+qed
+
+lemma leading_ref' [rlaw]: "spec p r \<le> F \<Longrightarrow> spec p q \<le> F; spec r q"
+  apply (rule leading_ref[rotated])
+  apply assumption
+  apply (rule sequence_ref)
+done
+
+lemma following_assignment_ref [rlaw]: "q' \<subseteq> subst_pred q v m \<Longrightarrow> spec p q \<le> spec p q'; assign v m"
+  by (auto intro: following_ref mptran rlaw)
+
+lemma leading_assignment_ref [rlaw]: "p \<subseteq> subst_pred p' v m \<Longrightarrow> spec p q \<le> assign v m; spec p' q"
+  by (auto intro: leading_ref rlaw)
+
+
+lemma iso_while_spec [mptran]: "mono (\<lambda>p. while b (spec p i))"
+proof (auto simp: mono_def)
+  fix x y :: "'a pred" assume "x \<le> y"
+  moreover have "mono (spec x i)"
+    by (simp add: spec_mono)
+  moreover have "(spec x i) \<le> (spec y i)"
+    by (simp add: calculation(1) weaken_pre)
+  ultimately show "while b (spec x i) \<le> while b (spec y i)"
+    by (auto intro!: iso_while)
+qed
+
+lemma while_ref_tactic [rlaw]: "\<lbrakk>i \<sqinter> b \<le> p'; p \<le> i; i - b \<le> q\<rbrakk> \<Longrightarrow> spec p q \<le> while b (spec p' i)"
+proof -
+  assume "p \<le> i" "i - b \<le> q" and assm: "i \<sqinter> b \<le> p'"
+  hence "spec p q \<le> spec i (i \<sqinter> -b)"
+    by (metis diff_eq weaken_and_strengthen)
+  also have "... \<le> while b (spec (i \<sqinter> b) i)"
+    by (simp add: while_ref)
+  also have "... \<le> while b (spec p' i)"
+    using assm by (auto intro!: monoD mptran)
+  finally show ?thesis
+    by simp
+qed
+
+
+lemma [rlaw]: "mono R \<Longrightarrow> (\<And>x. spec (P x) (Q x) \<le> R) \<Longrightarrow> spec (EXS x. P x) (EXS y. Q y) \<le> R"
+  apply (subst ht_spec_eq[symmetric])
+  apply simp
+  apply (rule hl_exs2)
+  apply simp
+by (simp add: ht_spec_eq)
+ 
+lemma dispose_ref [rlaw]: "spec ((e \<mapsto> n) * r) r \<le> dispose e"
+  by (simp add: mono_dispose sl_dispose_alt specI)
+(*
+lemma lookup_ref2 [rlaw]: "vars2 v_upd v v' \<Longrightarrow> vars3 v_upd v' \<Longrightarrow> free v_upd e \<Longrightarrow> spec ((e \<mapsto> v') * r) (<{s. v s = v' s}>  * (e \<mapsto> v') * r) \<le> lookup v_upd e"
+  sorry
+*)
+
+lemma frame_ref [rlaw]: "mono x \<Longrightarrow> local x r \<Longrightarrow> spec p q \<le> x \<Longrightarrow> spec (p * r) (q * r) \<le> x"
+  using ht_spec_eq sl_frame by blast
+
+lemma frame_ref2 [rlaw]: "mono x \<Longrightarrow> local x r \<Longrightarrow> spec p q \<le> x \<Longrightarrow> spec (r * p) (r * q) \<le> x"
+  by (simp add: frame_ref sep_comm)
+
+lemma mutation_ref [rlaw]: "spec ((e \<mapsto> n) * r) ((e \<mapsto> e') * r) \<le> mutation e e'"
+  apply (rule frame_ref)
+  apply (rule mptran | rule lptran)+
+  apply (subst ht_spec_eq[symmetric])
+  apply (rule mptran)
+  apply (rule sl_mut_local')
+done
+
+lemma mutation_ref2 [rlaw]: "spec ((i \<mapsto> a, b) * r) ((i \<mapsto> a, e) * r) \<le> mutation (\<lambda>s. i s + 1) e"
+  apply (rule frame_ref)
+  apply (rule mptran | rule lptran)+
+  apply (simp add: doublet_def)
+  apply (rule frame_ref2)
+  apply (rule mptran | rule lptran)+
+  apply (subst ht_spec_eq[symmetric])
+  apply (rule mptran)
+  apply (rule sl_mut_local')
+done
+
+lemma seq_assoc: "(x ; y); z = x; (y; z)"
+  by (auto simp: seq_def)
+
+lemma [rlaw]: "mono x \<Longrightarrow> y \<le> z \<Longrightarrow> x ; y \<le> x ; z"
+  apply (auto simp: seq_def)
+by (metis following_ref order_refl seq_def)
+
+declare iso_while [rlaw]
+
+(*
+lemma [rlaw]: "x \<le> y \<Longrightarrow> while b x \<le> while b y"
+  apply (auto simp: while_def)
+*)
+lemma lookup_ref [rlaw]: "\<forall>s x. k (k_update (\<lambda>_. x) s) = x \<Longrightarrow> \<forall>s x. i (k_update (\<lambda>_. x) s) = i s \<Longrightarrow> \<forall>x. subst_pred (R k) k_update (\<lambda>_. x) = R (\<lambda>_. x) \<Longrightarrow> 
+            spec (EXS x. (i \<mapsto> (\<lambda>_. a), (\<lambda>_. x)) * R (\<lambda>_. x))
+                ((i \<mapsto> (\<lambda>_. a), k) * R k)
+               \<le> lookup k_update (\<lambda>s. i s + 1)"
+               apply (rule specI)
+               apply (rule mptran)+
+               apply (rule hl_pre[rotated])
+               apply (rule sl_lookup2)
+               apply (rule mono_exs2)
+               apply sep_normal
+               apply (rule reynolds5')
+               apply (metis (no_types, lifting) bbi.Sup.qisol bbi.mult.left_commute top_greatest)
+               apply simp
+done
+
+
+(***********************************************************************************************)
+
+text {* \emph{morgan} tactic *}
+
+method morgan_step uses simp ref = 
+  (assumption | subst sep_assoc | subst seq_assoc | rule ref rlaw mptran)
+
+method morgan uses simp ref = 
+  (morgan_step simp: simp ref: ref; (morgan simp: simp ref: ref)?)+
+
+
+
+end
