SL/StoreHeapModel.thy
@@ -69,14 +69,14 @@ lemma local_eq: "local (basic f) R \<longleftrightarrow> basic_local f R"
   by (force simp: local_def basic_local_def basic_def sep_def)
 
 lemma local_assign: "free_pred v R \<Longrightarrow> local (assign v t) R"
-  by (force simp: local_eq basic_local_def assign_def basic_def sep_def valid_mem_def)
+  by (force simp: subst_pred_def local_eq basic_local_def assign_def basic_def sep_def valid_mem_def)
 
 lemma local_lookup [lptran]: "free_pred u R \<Longrightarrow> local (lookup u t) R"
   apply (auto simp: local_eq basic_local_def lookup_def basic_def sep_def valid_mem_def)
   apply (rule_tac x=h1 in exI)
   apply (rule_tac x=h2 in exI)
   apply (subgoal_tac "the ((h1 ++ h2) (t s)) = y")
-  apply force
+  apply (force simp: subst_pred_def)
   by (simp add: heap_divider)
 
 lemma local_mutation [lptran]: "local (mutation e t) R"
@@ -91,15 +91,16 @@ done
 lemma "Q n \<Longrightarrow> P (SOME n. Q n) \<Longrightarrow> P n"
 nitpick oops
 
-lemma local_cons [lptran]: "free_pred v R \<Longrightarrow> local (cons u t) R"
+find_theorems name: ex_new_if_finite
+
+lemma "dom h \<noteq> UNIV \<Longrightarrow> \<exists>n. n \<notin> dom h"
+  apply auto
+done
+
+lemma local_cons [lptran]: "\<forall>h. \<exists>n. n \<notin> dom h \<Longrightarrow> local (cons u t) R"
 apply (simp add: cons_def local_eq basic_local_def)
 apply auto
-apply (rule_tac someI2_ex)
-defer
-apply (erule conjE)
-apply (subst (asm) someI_ex) 
 oops
-
 
 
 lemma local_dispose [lptran]: "local (dispose e) R"
@@ -123,15 +124,18 @@ lemma hl_basic [sl]: "P \<subseteq> {s. f s in Q} \<Longrightarrow> ht P (basic 
   by (auto simp: ht_def basic_def seq_def)
 
 lemma hl_assign [sl]: "P \<subseteq> subst_pred Q z_upd t \<Longrightarrow> ht P (assign z_upd t) Q"
-  by (auto simp: assign_def valid_mem_def intro!: sl)
+  by (auto simp: assign_def subst_pred_def valid_mem_def intro!: sl)
 
 lemma sl_mut_local [sl]: "ht (e \<mapsto> -) (mutation e e') (e \<mapsto> e')"
+  by (auto simp: mutation_def valid_mem_def any_singleton_def singleton_def intro!: sl)
+
+lemma sl_mut_local' [sl]: "ht (e \<mapsto> n) (mutation e e') (e \<mapsto> e')"
   by (auto simp: mutation_def valid_mem_def any_singleton_def singleton_def intro!: sl)
 
 lemma sl_mut_global [sl]: "ht ((e \<mapsto> -) * r) (mutation e e') ((e \<mapsto> e') * r)"
   by (auto intro: sl lptran)
 
-lemma sl_mut [sl]: "ht ((e \<mapsto> -) * ((e \<mapsto> e') -* r)) (mutation e e') r"
+lemma sl_mut: "ht ((e \<mapsto> -) * ((e \<mapsto> e') -* r)) (mutation e e') r"
   apply (rule hl_post[where Q'="(e \<mapsto> e') * ((e \<mapsto> e') -* r)"])
   by (auto simp: Assertions.bbi.sep_impl_annil1 intro!: sl_mut_global mptran)
 
@@ -140,6 +144,13 @@ lemma sl_dipose_local [sl]: "ht (e \<mapsto> -) (dispose e) (emp)"
 
 lemma sl_dispose [sl]: "ht ((e \<mapsto> -) * r) (dispose e) r"
   by (subst bbi.mult_1[symmetric], (rule sl | rule lptran)+)
+
+lemma sl_dispose_alt [sl]: "ht ((e \<mapsto> n) * r) (dispose e) r"
+  apply (rule hl_pre)
+  defer
+  apply (rule sl_dispose)
+  apply (rule bbi.qiso)
+  by (auto simp: any_singleton_def singleton_def)
 
 lemma sl_alloc_local [sl]: "free u_upd e \<Longrightarrow> vars1 u_upd u \<Longrightarrow> ht emp (cons u_upd e) (u \<mapsto> e)"
   apply (auto simp: cons_def emp_def valid_mem_def singleton_def intro!: sl)
@@ -160,16 +171,20 @@ lemma sl_lookup_local [sl]: "vars2 v_upd v v' \<Longrightarrow> vars3 v_upd v' \
     ht (e \<mapsto> v') (lookup v_upd e) ((v \<Midarrow> v') \<sqinter> (e \<mapsto> v'))"
   by (auto simp: lookup_def valid_mem_def singleton_def intro!: sl)
 
+lemma sl_lookup_global [sl]: "vars2 v_upd v v' \<Longrightarrow> vars3 v_upd v' \<Longrightarrow> free v_upd e \<Longrightarrow> 
+    ht ((e \<mapsto> v') * r) (lookup v_upd e) ((<{s. v s = v' s}> * (e \<mapsto> v')) * r)"
+oops
+
 lemma sl_lookup_lkl [sl]: "vars1 v_upd v \<Longrightarrow> vars3 v_upd v'' \<Longrightarrow> free v_upd e \<Longrightarrow>
     ht ((v \<Midarrow> v') \<sqinter> (e \<mapsto> v'')) (lookup v_upd e) ((v \<Midarrow> v'') \<sqinter> (subst e v_upd v' \<mapsto> v))"
   by (auto simp: lookup_def valid_mem_def singleton_def intro!: sl)
 
-lemma sl_lookup [sl]: "ht (EXS v'. (e \<mapsto> v') * ((e \<mapsto> v') -* (subst_pred r v_upd v'))) (lookup v_upd e) r"
+lemma sl_lookup: "ht (EXS v'. (e \<mapsto> v') * ((e \<mapsto> v') -* (subst_pred r v_upd v'))) (lookup v_upd e) r"
   apply (auto simp: lookup_def intro!: sl)
   apply (subgoal_tac "(a, b) \<in> subst_pred r v_upd x")
   prefer 2
   using bbi.sep_impl_annil1 apply blast
-  apply auto
+  apply (auto simp: subst_pred_def)
   apply (clarsimp simp: valid_mem_def)
   prefer 2
   apply (clarsimp simp: valid_mem_def)
@@ -182,8 +197,25 @@ lemma sl_lookup [sl]: "ht (EXS v'. (e \<mapsto> v') * ((e \<mapsto> v') -* (subs
   apply auto
   by (simp add: domI ortho_def)
 
+lemma sl_lookup2: "ht (EXS v'. (e \<mapsto> #v') * ((e \<mapsto> #v') -* (subst_pred r v_upd #v'))) (lookup v_upd e) r"
+  apply (auto simp: lookup_def intro!: sl)
+  apply (subgoal_tac "(a, b) \<in> subst_pred r v_upd #x")
+  prefer 2
+  using bbi.sep_impl_annil1 apply blast
+  apply (auto simp: subst_pred_def)
+  apply (clarsimp simp: valid_mem_def)
+  prefer 2
+  apply (clarsimp simp: valid_mem_def)
+  apply (clarsimp simp: sep_def singleton_def)
+  apply (rule_tac x="x" in exI)
+  apply (simp add: heap_divider)
+  apply (subgoal_tac "y = x")
+  apply simp
+  apply (clarsimp simp: sep_def singleton_def)
+  apply auto
+  by (simp add: domI ortho_def)
 
-lemma sl_lookup_alt [sl]: "ht (EXS v'. (e \<hookrightarrow> v') \<sqinter> (subst_pred r v_upd v')) (lookup v_upd e) r"
+lemma sl_lookup_alt: "ht (EXS v'. (e \<hookrightarrow> v') \<sqinter> (subst_pred r v_upd v')) (lookup v_upd e) r"
   apply (rule hl_pre)
   prefer 2
   apply (rule sl_lookup)
@@ -200,5 +232,49 @@ lemma sl_lookup_alt [sl]: "ht (EXS v'. (e \<hookrightarrow> v') \<sqinter> (subs
   apply (rule reynolds5)
 done
 
+lemma sl_lookup_alt2: "ht (EXS v'. (e \<hookrightarrow> #v') \<sqinter> (subst_pred r v_upd #v')) (lookup v_upd e) r"
+  apply (rule hl_pre)
+  prefer 2
+  apply (rule sl_lookup)
+  apply (rule Collect_mono)
+  apply (rule impI)
+  apply (erule exE)
+  apply (rule_tac x="#xa" in exI)
+  apply (rule impE)
+  prefer 2
+  apply assumption
+  prefer 2
+  apply assumption
+  apply (rule in_mono)
+  apply (rule reynolds5)
+done
 
+lemma sl_lookup_alt3: "p \<subseteq> (EXS v'. (e \<hookrightarrow> #v') \<sqinter> (subst_pred q v_upd #v')) \<Longrightarrow> ht p (lookup v_upd e) q"
+apply (rule hl_pre)
+apply assumption
+apply (rule sl_lookup_alt2)
+done
+
+named_theorems hl_rules
+
+(*
+method hoare_init uses simp = 
+  ((rule allI | rule ballI | subst simp | subst fst_conv | subst snd_conv)+)?
+*)
+
+method hoare_init uses simp = 
+  ((subst simp | subst fst_conv | subst snd_conv)+)?
+
+method hoare_step uses simp hl = 
+  (hoare_init simp: simp, (assumption | rule subset_refl | rule mptran  | rule lptran | rule hl sl | rule allI | rule ballI | sep_normal | rule hl_exs))
+
+method hoare_ind uses simp hl = 
+  (hoare_step simp: simp hl: hl; (hoare_ind simp: simp hl: hl)?)+
+
+method hoare uses simp hl = 
+  (hoare_init simp: simp; (hoare_ind simp: simp hl: hl)?)
+
+method hl_aux uses rule =
+  (rule allI, rule rule; ((erule_tac x=u in allE)+, assumption))
+  
 end
